#math #compnum 
## adding and subtracting
in [[rectangular form]]
$(x_1+jy_1)\pm(x_2+jy_2)=(x_1\pm x_2)+j(y_1\pm y_2)$
what if in [[exponential form]]
convert to [[rectangular form]]
$A_3e^{j\phi_3}=x_3+jy_3$
then add/subtract as before

## Multiplying/Dividing
### easy in [[exponential form]]
[[rectangular form]] works but is tedious and prone to error
$A_3e^{j\phi_3}*A_4e^{j\phi_4}=(A_3*A_4)(e^{j\phi_3}*e^{j\phi_4})=A^3A^4e^{j(\phi_3+\phi_4)}$
$A_3e^{j\phi_3}/A_4e^{j\phi_4}=(A_3/A_4)(e^{j\phi_3}*e^{-j\phi_4})=A^3/A^4e^{j(\phi_3-\phi_4)}$
the [[amplitude]] of a product is the product of the [[amplitude]]
the [[phase]] of a product is the sum of the [[phases]]
### just by j
$j(3+j4)=-4+j3$
$j(10e^{j120^o})=e^{j90}+10e^{j120^o}=10e^{j210^o}$
mult rotates by 90 degrees positively
divide rotates by 90 degrees negatively
easiest in [[exponential form]] still

### Negate (multiply by -1)
$-10e^{j120^o}=-1*10e^{j120^o}=e^{j180^o}*10e^{j120^o}=10e^{j300^o} = 10e^{-j60^o}$
## Special Cases (worth memorize)
$j = 0+j1 = e^{j90^o} =1 \angle \pi /2$
$-1 = -1+j0 = e^{j180^o} = 1\angle \pi$
$-j = 0-j1 = e^{j270^o}=1\angle 3\pi/2$
$1 = 1+j0 = e^{j0^o}=1\angle2\pi$
![[Pasted image 20230909183411.png]]

