#Conttime 
## Definition
The convolution of two functions $f(t)$ and $g(t)$ is defined as:

$$ (f*g)(t) = \int_{-\infty}^{\infty} f(\tau)g(t-\tau)d\tau $$
The convolution of two functions, denoted as $(f*g)(t)$, is a way to combine the two functions together. It involves taking the [[integral]] (or area under the curve) of the product of one function, $f(\tau)$, and another function, $g(t-\tau)$, as $\tau$ goes from negative infinity to positive infinity. This [[integral]] essentially represents how much one function "overlaps" with the other function at each point in time. The result of this operation is a new function that describes how the two original functions interact with each other.
## Key Theorem: Convolution Theorem
The convolution theorem states that the [[Fourier transform]] of the convolution of two functions is equal to the pointwise product of their Fourier transforms. Mathematically, it can be expressed as:

$$ \mathcal{F}\{f*g\} = \mathcal{F}\{f\} \cdot \mathcal{F}\{g\} $$

## Example
Let's consider two functions $f(t) = e^{-t}$ and $g(t) = t$. To find their convolution, we can use the definition of convolution:

$$ (f*g)(t) = \int_{0}^{t} e^{-\tau}\tau d\tau $$

To solve the [[integral]] $\int_{0}^{t} e^{-\tau}\tau d\tau$, we can use [[integration by parts]]. 

Let's set $u = \tau$ and $dv = e^{-\tau} d\tau$. Then, we have $du = d\tau$ and $v = -e^{-\tau}$.

Using the formula for [[integration by parts]]:

$$ \int u dv = uv - \int v du $$

Substitute in our values for $u$, $v$, $du$, and $dv$:

$$ \int_{0}^{t} e^{-\tau}\tau d\tau = -e^{-\tau}\tau|_{0}^{t} - \int_{0}^{t} -e^{-\tau}d\tau $$

Evaluate the first term at the limits of [[integration]]:

$$ (-e^{-t}t + e^0*0) + \int_{0}^{t} e^{-\tau}d\tau $$

Simplify further:

$$ -e^{-t}t + 1 - e^0*0 $$

This simplifies to:

$$ 1 - (1+t)e^{-t} $$

Therefore, the convolution of the functions $f(t) = e^{-t}$ and $g(t) = t$ is given by $(f*g)(t) = 1 - (1+t)e^{-t}$.

Sure! Let's consider two step functions $f(t)$ and $g(t)$ with partial overlap. 

Suppose $f(t)$ is a [[step function]] defined as:

$$ f(t) = \begin{cases} 
      0 & t < 0 \\
      1 & t \geq 0 
   \end{cases}
$$

And let $g(t)$ be another [[step function]] defined as:

$$ g(t) = \begin{cases} 
      0 & t < a \\
      1 & t \geq a 
   \end{cases}
$$

where $a$ is some positive constant.

To identify the partial overlap between these two step functions, we need to find the range of values for which both functions are non-zero. In this case, the partial overlap occurs when $t \geq a$, since both functions are equal to 1 for this range of values.

To find the convolution $(f*g)(t)$, we can use the definition of convolution:

$$ (f*g)(t) = \int_{-\infty}^{\infty} f(\tau)g(t-\tau)d\tau $$

Since $f(\tau)$ is only non-zero for $\tau \geq 0$ and $g(t-\tau)$ is only non-zero for $\tau \leq t$, the [[integral]] simplifies to:

$$ (f*g)(t) = \int_{0}^{t} g(t-\tau)d\tau $$

For the given step functions, this [[integral]] can be split into two cases depending on the value of $t$ relative to $a$:

1. If $t < a$: The [[integral]] becomes:

$$ (f*g)(t) = \int_{0}^{t} g(t-\tau)d\tau = 0 $$

since $g(t-\tau)$ is zero for all values of $\tau$ in this range.

2. If $t \geq a$: The [[integral]] becomes:

$$ (f*g)(t) = \int_{0}^{a} g(t-\tau)d\tau + \int_{a}^{t} g(t-\tau)d\tau $$

In this case, both integrals will contribute to the overall convolution since there is an overlap between the two step functions.

By evaluating these integrals, you can find the expression for $(f*g)(t)$ when there is partial overlap between two step functions.
